Ring scheduler for message passing

examples/Queue.v
@@ -14,12 +14,13 @@ From CTree Require Import
 
 From ExtLib Require Export
   Structures.MonadState
-  Data.Monads.StateMonad
-  Structures.Monad.
+  Data.Monads.StateMonad.
 
 From Coq Require Import
   Lia
   List.
+
+From ExtLib Require Import RelDec.
 
 Generalizable All Variables.
 
@@ -51,7 +52,9 @@ Arguments push /.
 Arguments pop /.
 
 Section QueueEx.
-  Context {S: Type}.
+  Context {S: Type} {HDec: RelDec (@eq S)} {HCor: RelDec_Correct HDec}.
+  Infix "=?" := (rel_dec) (at level 75).
+  
   (* Ex1: Drain a queue *)
   Definition drain: ctree (queueE S) unit :=
     iter (fun _ =>
@@ -108,7 +111,7 @@ Section QueueEx.
   Theorem drain_af_pop: forall (s: S) q,
       <( {interp_state h_queueE drain (q ++ [s])}, Pure |=
          AF finishW \v l, v = s /\ l = @nil S )>.
-  Proof.
+  Proof with eauto with ctl.
     intros.
     apply af_iter_state_list
       with (Ri:=fun '(tt) w l =>
@@ -133,15 +136,16 @@ Section QueueEx.
     - (* l = [] *)
       inv Hd; cbn.
       + destruct Hw, x; cbn in *; inv H.
-      + rewrite bind_ret_l, bind_tau.
-        apply af_tau.
+      + destruct e, v.
+        subst.
+        rewrite bind_ret_l, bind_guard.
+        apply af_guard.
         rewrite interp_state_ret, bind_ret_l.
         cbn.
         rewrite interp_state_ret.
         next; left.
-        apply ax_finish.
+        apply ax_done; split...
         do 2 eexists; intuition.
-        destruct e, v; subst; auto.
     - (* l = h :: ts *)
       cbn.
       rewrite bind_trigger, bind_vis.      
@@ -149,13 +153,13 @@ Section QueueEx.
       + apply can_step_vis; intuition.
       + intros t' w' TR.
         apply ktrans_vis in TR as (x & -> & <- & _).        
-        rewrite bind_ret_l, bind_tau.
-        apply af_tau.
+        rewrite bind_ret_l, bind_guard.
+        apply af_guard.
         rewrite interp_state_ret, bind_ret_l.
         cbn.
         rewrite interp_state_ret.
         next; left.
-        apply ax_finish; cbn; destruct x; intuition. 
+        apply ax_done; cbn; destruct x; intuition. 
         inv Hd.
         * destruct Hw as [[|h' ts'] Hw];
             apply list_app_cons in Hw as (-> & ->); cbn; auto.
@@ -168,12 +172,125 @@ Section QueueEx.
           -- now (exists (s2 :: x)).
   Qed.       
 
-  Theorem rotate_af_pop: forall (t f: S) (Htf: t <> f) q,
-      <( {interp_state h_queueE (rotate f) (q ++ [t])}, Pure |=
-         AF finishW \v l, v = t /\ Forall (eq f) l )>.
+  Record ghostS :=
+   mkGhost {
+      elem : S;
+      dist : nat;
+   }.
+
+  Fixpoint index(l: list S)(s: S): option nat :=
+    match l with
+    | h :: ts =>
+        if h =? s then
+          Some (List.length ts)
+        else
+          index ts s
+    | nil => None
+    end.
+
+
+  (* Needle to look for *)
+  Context (t: S) (f: S) (Htf: f <> t).
+
+  Lemma index_last_S: forall l,
+      index (l ++ [f]) t = option_map Datatypes.S (index l t).
   Proof.
+    induction l; cbn.
+    - eapply rel_dec_neq_false in Htf; eauto.
+      now rewrite Htf.
+    - destruct (a =? t) eqn:Ha.
+      + rewrite app_length; cbn.
+        rewrite PeanoNat.Nat.add_1_r.
+        reflexivity.
+      + apply IHl.
+  Qed.
+
+  Definition h_ghostE: queueE S ~> stateT (list S) (ctree (writerE ghostS)) :=
+    h_writerA
+      (* queue semantics *)
+      (h_state h_queueE_sem)
+      (* queue instrumentation, observe [Pop] + ghost state *)
+      (fun (e: queueE S) (v: encode e) (q: list S) =>
+         match e return encode e -> option ghostS with
+         | Pop => fun x: option S =>
+                   match x with
+                   | Some x =>
+                       match index q t with
+                       | Some i => Some (mkGhost x i)
+                       | None => None
+                       end
+                   | None => None
+                   end
+         | Push x => fun _ => None                      
+         end v).
+
+
+  Theorem rotate_af_pop: forall q,
+      <( {interp_state h_ghostE (rotate f) (q ++ [t])}, Pure |=
+           AF finishW \g l,
+             g.(elem) = t /\ g.(dist) = 0 /\ Forall (eq f) l )>.
+  Proof with eauto with ctl.
     intros.
-    Print rotate.
+    apply af_iter_state_list
+      with (Ri:=fun '(tt) w l =>
+                  not_done w /\
+                  match w with
+                  | Obs (Log g) tt =>
+                      length l = length q /\
+                        index l t = Some g.(dist)
+                  | _ => length l = length q /\
+                          index l t = Some (length l)
+                  end); [|eauto with ctl].
+    intros [] w l [Hw H'].    
+    rewrite interp_state_bind.
+    unfold pop, push, trigger.
+    rewrite interp_state_vis, bind_bind.
+    unfold runStateT, h_queueE; cbn.
+    rewrite bind_bind.
+    resum.
+    rewrite ?bind_ret_l, bind_guard.
+    apply af_guard.
+    rewrite interp_state_ret, bind_ret_l.
+    rewrite interp_state_bind, interp_state_vis.
+    rewrite bind_bind.
+    unfold runStateT; cbn.
+    rewrite bind_bind.
+    resum.
+    rewrite bind_ret_l.
+    destruct l as [|h ts]; cbn.
+    - (* l = [] *)
+      rewrite bind_ret_l, bind_guard.
+      apply af_guard.
+      rewrite interp_state_ret, bind_ret_l.
+      cbn.
+      rewrite interp_state_ret.
+      next; left.
+      apply ax_done.
+      intuition.
+      inv Hw.
+      + destruct H'; cbn in *.
+        inv H0.
+      + destruct v, e.
+        cbn in *.
+        destruct H'; inv H0.
+    - (* l = h::ts *)
+      cbn.
+      rewrite index_last_S.
+      inv Hw; cbn in H'.
+      + destruct H'.
+        destruct (h =? t) eqn:Hh.
+        * inv H0; lia.
+        * rewrite H0; cbn.
+          rewrite bind_trigger, bind_vis.
+          next; right.
+          next; split.
+          -- apply can_step_vis...
+          -- intros t' w' TR.
+             apply ktrans_vis in TR as ([] & -> & <- & _).
+             rewrite bind_ret_l, bind_guard, af_guard,
+               interp_state_ret, bind_ret_l. 
+             cbn.
+             rewrite interp_state_ret.
   Admitted.
 End QueueEx.
   
