theories/Events/NetE.v
@@ -23,68 +23,25 @@ Set Implicit Arguments.
 Generalizable All Variables.
 
 (*| Unique thread identifiers |*)
-Notation uid n := (fin n).
+Notation fin' n := (fin (S n)).
+Notation vec' n t := (vec (S n) t).
 
 (*| Message passing algebraic effects |*)
 Section Messaging.
   Context (n: nat) (T: Type).
-  Notation uid := (uid n).
 
   (*| Network effects |*)
   Inductive netE: Type :=
-  | Recv(me: uid)
-  | Send(me to: uid)(msg: T).
+  | Recv
+  | Send(to: fin' n)(msg: T).
 
   #[global] Instance encode_netE: Encode netE :=
     fun e => match e with
-          | Recv _ => option T
-          | Send _ _ _ => unit
+          | Recv => option T
+          | Send _ _ => unit
           end.
 
 End Messaging.
 
 Arguments Recv {n} {T}.
 Arguments Send {n} {T}.
-
-(*| Many interpretations for network effects. |*)
-
-(*| Bidirectional queues (input, output) interpretation
-  of an event [netE] |*)
-Section Messaging.
-  Import MonadNotation.
-  Local Open Scope monad_scope.
-
-  Context (n: nat) (T: Type).
-  Notation uid := (uid n).
-  Notation LQs := (list T * list (uid * T)) (only parsing).
-  Notation VQs := (vec n (list T)) (only parsing).
-  Notation netE := (netE n T).
-
-  Definition h_netE_l: netE ~> state LQs :=
-      fun e =>
-        '(inp, out) <- get ;;
-        match e return state LQs (encode e) with
-        | Recv me =>
-            match inp with
-            | [] => ret None
-            | msg :: ts => put (ts, out) ;; ret (Some msg)
-            end
-        | Send _ to msg => put (inp, out ++ [(to, msg)])
-        end.
-
-  Definition h_netE_v: netE ~> state VQs :=
-    fun e =>
-        qs <- get;;
-        match e return state VQs (encode e) with
-        | Recv i =>
-            match Vector.nth qs i with
-            | [] => ret None
-            | msg :: ts =>
-                put (nth_map qs i (fun _ => ts));;
-                ret (Some msg)
-            end
-        | Send i to msg => put (nth_map qs to (fun q => q ++ [msg]))
-        end.
-
-End Messaging.
-
